\documentclass[11pt]{article}
% \usepackage{times}
\usepackage{palatino}
\usepackage{colortbl}
\usepackage{enumitem}

\renewcommand{\baselinestretch}{1.2} 
\setlength{\topmargin}{-1.0in}
\setlength{\textwidth}{6.5in}
\setlength{\oddsidemargin}{0.0in}
\setlength{\textheight}{10.1in}

\newlength{\pagewidth}
\setlength{\pagewidth}{6.5in}
\pagestyle{empty}

\def\pp{\par\noindent}

\special{papersize=8.5in,11in}


\begin{document}
\noindent 
Tony Li \\
CSE150 \\
HW01a \\\\
%=========================================Problem 1=====================================================
	\textbf{\underline{Problem 1:}}


	Write P $\Rightarrow$ Q using $\vee$ and $\sim$. Show that your two representations are equivalent.
	\\
	\\
	
	\begin{minipage}{0.5\textwidth}
		\begin{tabular}{||c c c c c||} 
 		\hline
 		P & Q & $\sim$P & P$\Rightarrow$Q & $\sim$P $\vee$ Q\\ [0.5ex] 
 		\hline\hline
 		T & T & F & T & T\\ 
 		\hline
 		T & F & F & F & F\\
 		\hline
 		F & T & T & T & T\\
 		\hline
 		F & F & T & T & T\\
 		\hline
		\end{tabular}
	\end{minipage}
	\begin{minipage}{0.5\textwidth}
	
		\begin{tabular}{|c|}
		\arrayrulecolor{red}\hline
		$\sim$P $\vee$ Q\\[0.5ex]
		\hline
		\end{tabular}
	\end{minipage}\\\\

%=========================================Problem 2=====================================================
	\noindent
	\textbf{\underline{Problem 2:}} 


	Prove that the propositional formulas 
	\begin{center}
		P $\vee$ Q $\vee$ R
	\end{center}

	and
		
	\begin{center}
		(P $\wedge \sim$ Q) $\vee$ (Q $\wedge \sim$ R) $\vee$ (R $\wedge \sim$ P) $\vee$ (P $\wedge$ Q $\wedge$ R) 
	\end{center}

	are equivalent.
	\\\\
	\begin{tabular}{|c c c c c c !{\color{red}\vrule} c !{\color{red}\vrule} c c c c|} 
	\hline
	P & Q & R & $\sim$P & $\sim$Q & $\sim$R & P $\vee$ Q $\vee$ R & P $\wedge \sim$Q & Q $\wedge \sim$R & R $\wedge \sim$P & P $\wedge$ Q $\wedge$ R \\ [0.5ex] 
 		\hline\hline
	T & T & T & F & F & F & T & F & F & F & T \\
	T & T & F & F & F & T & T & F & T & F & F \\
	T & F & T & F & T & F & T & T & F & F & F \\
	T & F & F & F & T & T & T & T & F & F & F \\
	F & T & T & T & F & F & T & F & F & T & F \\
	F & T & F & T & F & T & T & F & T & F & F \\
	F & F & T & T & T & F & T & F & F & T & F \\
	F & F & F & T & T & T & F & F & F & F & F \\
	\hline
	\end{tabular} 

	\noindent
	\begin{tabular}{|c|}
		\arrayrulecolor{red}\hline
		\hline
		(P $\wedge \sim$ Q) $\vee$ (Q $\wedge \sim$ R) $\vee$ (R $\wedge \sim$ P) $\vee$ (P $\wedge$ Q $\wedge$ R) \\[0.5ex]
		\hline\hline
		T \\
		T \\
		T \\
		T \\
		T \\
		T \\
		T \\
		F \\
		\hline
		\end{tabular}\\\\\\\\


%=========================================Problem 3=====================================================
\noindent
	\textbf{\underline{Problem 3:}} 


	( a ) Write the biconditional ( $\Leftrightarrow$ ) using only implies ( $\Rightarrow$ ) and ( $\wedge$ ). Prove that the new version

 	is equivalent.

	\begin{minipage}{0.5\textwidth}
		\begin{tabular}{||c c c c c||} 
 		\hline
 		P & Q & P $\Rightarrow$ Q & Q$\Rightarrow$P & (P $\Rightarrow$ Q) $\wedge$ (Q$\Rightarrow$P)\\ [0.5ex] 
 		\hline\hline
 		T & T & T & T & T\\ 
 		\hline
 		T & F & F & T & F\\
 		\hline
 		F & T & T & F & F\\
 		\hline
 		F & F & T & T & T\\
 		\hline
		\end{tabular}
	\end{minipage}
	\begin{minipage}{0.5\textwidth}
	
		\begin{tabular}{|c|}
		\arrayrulecolor{red}\hline
		(P $\Rightarrow$ Q) $\wedge$ (Q$\Rightarrow$P)\\[0.5ex]
		\hline
		\end{tabular}
	\end{minipage}\\\\

	( b ) Write it using only $\vee$ and $\sim$. Show your derivation.
	
	\begin{enumerate}
		\item P $\Leftrightarrow$ Q
		\item (P $\Rightarrow$ Q) $\wedge$ (Q$\Rightarrow$P) \textit{[ by Problem 3a ]}
		\item ($\sim$P $\vee$ Q ) $\wedge$ ( $\sim$Q $\vee$ P ) \textit{[ by Problem 1]}
		\item $\sim$ ( $\sim$ ( $\sim$P $\vee$ Q ) ) $\vee$ $\sim$ ( $\sim$Q $\vee$ P ) ) \textit{[ by De Morgan's Laws ]}
	\end{enumerate}

	\begin{tabular}{|c|}
		\arrayrulecolor{red}\hline
		$\sim$ ( $\sim$ ( $\sim$P $\vee$ Q ) ) $\vee$ $\sim$ ( $\sim$Q $\vee$ P ) )\\[0.5ex]
		\hline
	\end{tabular}
		




 	
	

	
\end{document}